@prefix rdf: <http://www.w3.org/1999/02/22-rdf-syntax-ns#> .
@prefix rdfs: <http://www.w3.org/2000/01/rdf-schema#> .
@prefix bf: <http://id.loc.gov/ontologies/bibframe/> .
@prefix bflc: <http://id.loc.gov/ontologies/bflc/> .
@prefix owl: <http://www.w3.org/2002/07/owl#> .
@prefix skos: <http://www.w3.org/2004/02/skos/core#> .
@prefix dcterms: <http://purl.org/dc/terms/> .
@prefix foaf: <http://xmlns.com/foaf/0.1/> .
@prefix cc: <http://creativecommons.org/ns#> .

<http://id.loc.gov/ontologies/bflc/>
    cc:license <https://creativecommons.org/publicdomain/zero/1.0/> ;
    dcterms:creator [
        rdfs:resource "http://id.loc.gov/vocabulary/organizations/dlc"
    ] ;
    dcterms:issued "2022-10-06T12:00:00.000-05:00"^^<http://www.w3.org/2001/XMLSchema#dateTime> ;
    dcterms:modified "2022-10-07T12:17:40.528-04:00" ;
    dcterms:publisher [
        rdfs:resource "http://id.loc.gov/vocabulary/organizations/dlcmrc"
    ] ;
    dcterms:rights <https://creativecommons.org/publicdomain/zero/1.0/> ;
    a owl:Ontology ;
    rdfs:label "BIBFRAME vocabulary with LC extensions" ;
    owl:imports <http://id.loc.gov/ontologies/bibframe>, <http://id.loc.gov/vocabulary/relators> ;
    owl:ontologyIRI <http://id.loc.gov/ontologies/bflc/> ;
    owl:priorVersion <http://id.loc.gov/ontologies/bflc-1-2-0/> ;
    owl:versionIRI <http://id.loc.gov/ontologies/bflc-2-2-0/> ;
    owl:versionInfo "2.2.0"^^<http://www.w3.org/2001/XMLSchema#string> .

bflc:AppliesTo
    dcterms:modified "2017-02-02 (New)" ;
    a owl:Class ;
    rdfs:label "Applies to" ;
    skos:definition "The component of a resource to which a characteristic applies." .

bflc:CaptureStorage
    dcterms:modified "2019-05-20 (New [GH16])" ;
    a owl:Class ;
    rdfs:label "Capture and Storage Technique" ;
    rdfs:subClassOf bf:SoundCharacteristic ;
    skos:definition "Specifies the sound capture and storage technique used on a sound recording resource." .

bflc:CreatorCharacteristic
    dcterms:modified "2017-02-02 (New)" ;
    a owl:Class ;
    rdfs:label "Creator characteristic" ;
    skos:definition "Category to which the creators of the resource belong." .

bflc:DemographicGroup
    dcterms:modified "2017-02-02 (New)" ;
    a owl:Class ;
    rdfs:label "Demographic group" ;
    skos:definition "Characteristics of a group of agents." .

bflc:Deprecated
    dcterms:modified "2022-10-03 (New [GH6])" ;
    a owl:Class ;
    rdfs:label "Deprecated" ;
    skos:definition "The resource has been deprecated" .

bflc:EncodingLevel
    dcterms:modified "2017-02-02 (New)" ;
    a owl:Class ;
    rdfs:label "Encoding level" ;
    skos:definition "Designation of the fullness of the bibliographic description." .

bflc:GovernmentPubType
    dcterms:modified "2020-03-09 (New [GH10])" ;
    a owl:Class ;
    rdfs:label "Government Publication Type" ;
    skos:definition "Information recording that the resource is published or produced by or for an international, national, state, provincial, or local government agency, or by any subdivision of such a body." .

bflc:GrooveCutting
    dcterms:modified "2018-07-12 (New)" ;
    a owl:Class ;
    rdfs:label "Groove cutting" ;
    rdfs:subClassOf bf:SoundCharacteristic ;
    skos:definition "Kind of cutting of the grooves used on a disc whose sound reproduction process involves a cutting head inscribing a modulated groove into the surface of a rotating cylinder or disc." .

bflc:ImageBitDepth
    dcterms:modified "2017-02-02 (New)" ;
    a owl:Class ;
    rdfs:label "Image bit depth" ;
    rdfs:subClassOf bf:DigitalCharacteristic ;
    skos:definition "The number of bits used to represent each pixel in an image." .

bflc:MachineModel
    dcterms:modified "2017-02-02 (New)" ;
    a owl:Class ;
    rdfs:label "Model" ;
    rdfs:subClassOf bf:SystemRequirement ;
    skos:definition "Model of the computing device on which the resource operates." .

bflc:MetadataLicensor
    dcterms:modified "2017-02-02 (New)" ;
    a owl:Class ;
    rdfs:label "Metadata licensor" ;
    rdfs:subClassOf bf:Agent ;
    skos:definition "Organization that licenses the intellectual property rights to the data contained in the description." .

bflc:MovingImageTechnique
    dcterms:modified "2020-02-13 (New [GH9])" ;
    a owl:Class ;
    rdfs:label "Moving Image Technique" ;
    skos:definition "Specifies the technique used in creating motion in motion pictures or videorecordings." .

bflc:OperatingSystem
    dcterms:modified "2017-02-02 (New)" ;
    a owl:Class ;
    rdfs:label "Operating system" ;
    rdfs:subClassOf bf:SystemRequirement ;
    skos:definition "Software that directly operates a system's hardware and serves as a platform for applications." .

bflc:PrimaryContribution
    dcterms:modified "2017-02-02 (New)" ;
    a owl:Class ;
    rdfs:label "Primary contribution" ;
    rdfs:subClassOf bf:Contribution ;
    skos:definition "Contribution for which the agent is the name chosen as the name part of the name and title access point." .

bflc:ProgrammingLanguage
    dcterms:modified "2017-02-02 (New)" ;
    a owl:Class ;
    rdfs:label "Programming language" ;
    rdfs:subClassOf bf:SystemRequirement ;
    skos:definition "Name of the programming language associated with the data comprising the resource." .

bflc:Relation
    dcterms:modified "2017-02-02 (New)" ;
    a owl:Class ;
    rdfs:label "Relation" ;
    skos:definition "Connection between resources." .

bflc:Relationship
    dcterms:modified "2017-02-02 (New)" ;
    a owl:Class ;
    rdfs:label "Relationship" ;
    skos:definition "Resource and its connection to another resource." .

bflc:Relief
    dcterms:modified "2019-05-07 (New [GH13])" ;
    a owl:Class ;
    rdfs:label "Relief" ;
    skos:definition "Relief term specified on a cartographic resource" .

bflc:SerialPubType
    dcterms:modified "2020-03-18 (New [GH11])" ;
    a owl:Class ;
    rdfs:label "Serial Publication Type" ;
    skos:definition "Information recording the type of continuing resource." .

bflc:SeriesAnalysis
    dcterms:modified "2018-10-12 (New)" ;
    a owl:Class ;
    rdfs:label "Series analysis" ;
    rdfs:subClassOf bflc:SeriesTreatment ;
    skos:definition "A specific organization's analysis practice for a series named in the bf:title field for a work. May also contain the volumes/dates and/or the institution/copy identification to which the practice applies." .

bflc:SeriesClassification
    dcterms:modified "2018-10-12 (New)" ;
    a owl:Class ;
    rdfs:label "Series classification" ;
    rdfs:subClassOf bflc:SeriesTreatment ;
    skos:definition "A specific organization's classification practice for a series named in the bf:title field for a work. May also contain the volumes/dates and/or the institution/copy identification to which the practice applies." .

bflc:SeriesNumbering
    dcterms:modified "2018-10-12 (New)" ;
    a owl:Class ;
    rdfs:label "Series numbering" ;
    rdfs:subClassOf bflc:SeriesTreatment ;
    skos:definition "Sequential designation or numbering used in the bf:title field for a work." .

bflc:SeriesNumberingPeculiarities
    dcterms:modified "2018-10-12 (New)" ;
    a owl:Class ;
    rdfs:label "Series numbering peculiarities" ;
    rdfs:subClassOf bflc:SeriesTreatment ;
    skos:definition "Listing of irregularities in the report year coverage and/or numbering used in the bf:title field for a work. May also include a citation for the source of information." .

bflc:SeriesProvider
    dcterms:modified "2018-10-12 (New)" ;
    a owl:Class ;
    rdfs:label "Series provider" ;
    rdfs:subClassOf bflc:SeriesTreatment ;
    skos:definition "Place of publication and the name of the publisher/issuing body used in the bf:title field for a work." .

bflc:SeriesSequentialDesignation
    dcterms:modified "2018-10-12 (New)" ;
    a owl:Class ;
    rdfs:label "Series sequential designation" ;
    rdfs:subClassOf bflc:SeriesTreatment ;
    skos:definition "Beginning/ending date(s) of publication and/or sequential designations used in the bf:title field for a work. May also include a citation for the source of information." .

bflc:SeriesTracing
    dcterms:modified "2018-10-12 (New)" ;
    a owl:Class ;
    rdfs:label "Series tracing" ;
    rdfs:subClassOf bflc:SeriesTreatment ;
    skos:definition "A specific organization's tracing practice for a series named in the bf:title field for a work. May also contain the volumes/dates and/or the institution/copy identification to which the practice applies." .

bflc:SeriesTreatment
    dcterms:modified "2018-10-12 (New)" ;
    a owl:Class ;
    rdfs:label "Series treatment" ;
    skos:definition "Technical specification relating to the encoding of series data in a resource" .

bflc:TransliteratedTitle
    dcterms:modified "2018-07-12 (New)" ;
    a owl:Class ;
    rdfs:label "Transliterated title" ;
    rdfs:subClassOf bf:VariantTitle ;
    skos:definition "Title transliterated from one script to another." .

bflc:Uncontrolled
    dcterms:modified "2021-11-02 (New [GH15])" ;
    a owl:Class ;
    rdfs:label "Uncontrolled" ;
    skos:definition "Component of the resource that is not under authority control" .

bflc:aap
    dcterms:modified "2021-11-02 (New [GH2])" ;
    a owl:DatatypeProperty ;
    rdfs:comment "Used with Work, Instance or Item" ;
    rdfs:domain bf:WorkOrInstanceOrItem ;
    rdfs:label "Authorized access point" ;
    rdfs:range rdfs:Literal ;
    skos:definition "A text string that represents the label of the resource. It could be a name/title combination, but could also include additional fields to make it unique within the catalog." .

bflc:aap-normalized
    dcterms:modified "2021-11-02 (New [GH2])" ;
    a owl:DatatypeProperty ;
    rdfs:comment "Used with Work, Instance or Item" ;
    rdfs:domain bf:WorkOrInstanceOrItem ;
    rdfs:label "Normalized authorized access point" ;
    rdfs:range rdfs:Literal ;
    skos:definition "Normalized version of the authorized access point with spaces, capitalization, and punctuation removed." .

bflc:applicableInstitution
    dcterms:modified "2017-02-02 (New)" ;
    a owl:ObjectProperty ;
    rdfs:comment "Used with Work, Instance or Item" ;
    rdfs:domain bf:WorkOrInstanceOrItem ;
    rdfs:label "Applicable institution" ;
    rdfs:range bf:Agent ;
    skos:definition "Institutional location of a resource to which a particular piece of description applies." .

bflc:appliesTo
    dcterms:modified "2017-02-02 (New)" ;
    a owl:ObjectProperty ;
    rdfs:comment "Used with Work, Instance or Item" ;
    rdfs:domain bf:WorkOrInstanceOrItem ;
    rdfs:label "Applies to" ;
    rdfs:range bflc:AppliesTo ;
    skos:definition "The component of a resource to which a characteristic applies." .

bflc:catalogerId
    dcterms:modified "2018-07-12 (New)" ;
    a owl:DatatypeProperty ;
    rdfs:domain bf:AdminMetadata ;
    rdfs:label "Cataloger ID" ;
    rdfs:range rdfs:Literal ;
    skos:definition "ID of the cataloger who created or edited the description." .

bflc:creatorCharacteristic
    dcterms:modified "2017-02-02 (New)" ;
    a owl:ObjectProperty ;
    rdfs:comment "Used with Work, Instance or Item" ;
    rdfs:domain bf:WorkOrInstanceOrItem ;
    rdfs:label "Creator characteristic" ;
    rdfs:range bflc:CreatorCharacteristic ;
    skos:definition "Category to which the creators of the resource belong." .

bflc:demographicGroup
    dcterms:modified "2017-02-02 (New)" ;
    a owl:ObjectProperty ;
    rdfs:comment "Used with Work, Instance or Item" ;
    rdfs:domain bf:WorkOrInstanceOrItem ;
    rdfs:label "Demographic group" ;
    rdfs:range bflc:DemographicGroup ;
    skos:definition "Characteristics of a group of agents." .

bflc:distributionStatement
    dcterms:modified "2022-10-04 (New [GH18])" ;
    a owl:DatatypeProperty ;
    rdfs:comment "Used with Work, Instance or Item" ;
    rdfs:domain bf:WorkOrInstanceOrItem ;
    rdfs:label "Distribution statement" ;
    rdfs:range rdfs:Literal ;
    rdfs:subPropertyOf bflc:provisionActivityStatement ;
    skos:definition "Statement related to the distribution of the resource; usually transcribed." .

bflc:encodingLevel
    dcterms:modified "2017-02-02 (New)" ;
    a owl:ObjectProperty ;
    rdfs:domain bf:AdminMetadata ;
    rdfs:label "Encoding level" ;
    rdfs:range bflc:EncodingLevel ;
    skos:definition "Designation of the fullness of the bibliographic description." .

bflc:governmentPubType
    dcterms:modified "2020-03-09 (New [GH10])" ;
    a owl:ObjectProperty ;
    rdfs:comment "Used with Work, Instance or Item" ;
    rdfs:domain bf:WorkOrInstanceOrItem ;
    rdfs:label "Government publication type" ;
    rdfs:range bflc:GovernmentPubType ;
    skos:definition "Information recording that the resource is published or produced by or for an international, national, state, provincial, or local government agency, or by any subdivision of such a body." .

bflc:indexedIn
    dcterms:modified "2018-07-12 (New)" ;
    a owl:ObjectProperty ;
    rdfs:comment "Used with Work, Instance or Item" ;
    rdfs:domain bf:WorkOrInstanceOrItem ;
    rdfs:label "Indexed in" ;
    skos:definition "Citation to the resource where the material being described is indexed." .

bflc:manufactureStatement
    dcterms:modified "2022-10-04 (New [GH18])" ;
    a owl:DatatypeProperty ;
    rdfs:comment "Used with Work, Instance or Item" ;
    rdfs:domain bf:WorkOrInstanceOrItem ;
    rdfs:label "Manufacture statement" ;
    rdfs:range rdfs:Literal ;
    rdfs:subPropertyOf bflc:provisionActivityStatement ;
    skos:definition "Statement related to the manufacture of the resource; usually transcribed." .

bflc:marcKey
    dcterms:modified "2022-10-03 (New [GH7])" ;
    a owl:DatatypeProperty ;
    rdfs:comment "Used with Work, Instance or Item" ;
    rdfs:domain bf:WorkOrInstanceOrItem ;
    rdfs:label "MARC key for headings" ;
    rdfs:range rdfs:Literal ;
    skos:definition "String to store MARC data" .

bflc:metadataLicensor
    dcterms:modified "2017-02-02 (New)" ;
    a owl:ObjectProperty ;
    rdfs:domain bf:AdminMetadata ;
    rdfs:label "Metadata licensor" ;
    rdfs:range bflc:MetadataLicensor ;
    skos:definition "Organization that licenses the intellectual property rights to the data contained in the description." .

bflc:movingImageTechnique
    dcterms:modified "2020-02-13 (New [GH9])" ;
    a owl:ObjectProperty ;
    rdfs:comment "Used with Work, Instance or Item" ;
    rdfs:domain bf:WorkOrInstanceOrItem ;
    rdfs:label "Moving Image Technique" ;
    rdfs:range bflc:MovingImageTechnique ;
    skos:definition "Information recording the technique used in creating motion in motion pictures or videorecordings." .

bflc:name00MarcKey
    dcterms:modified "2017-02-02 (New)" ;
    a owl:DatatypeProperty ;
    rdfs:comment "Used with Work, Instance or Item" ;
    rdfs:domain bf:WorkOrInstanceOrItem ;
    rdfs:label "MARC key for X00 Names" ;
    rdfs:range rdfs:Literal ;
    skos:definition "String for personal name matching." .

bflc:name00MatchKey
    dcterms:modified "2017-02-02 (New)" ;
    a owl:DatatypeProperty ;
    rdfs:comment "Used with Work, Instance or Item" ;
    rdfs:domain bf:WorkOrInstanceOrItem ;
    rdfs:label "Match key for X00 Name" ;
    rdfs:range rdfs:Literal ;
    skos:definition "String for name matching." .

bflc:name10MarcKey
    dcterms:modified "2017-02-02 (New)" ;
    a owl:DatatypeProperty ;
    rdfs:comment "Used with Work, Instance or Item" ;
    rdfs:domain bf:WorkOrInstanceOrItem ;
    rdfs:label "MARC key for X10 Names" ;
    rdfs:range rdfs:Literal ;
    skos:definition "String for name matching." .

bflc:name10MatchKey
    dcterms:modified "2017-02-02 (New)" ;
    a owl:DatatypeProperty ;
    rdfs:comment "Used with Work, Instance or Item" ;
    rdfs:domain bf:WorkOrInstanceOrItem ;
    rdfs:label "Match key for X10 Name" ;
    rdfs:range rdfs:Literal ;
    skos:definition "String for name matching." .

bflc:name11MarcKey
    dcterms:modified "2017-02-02 (New)" ;
    a owl:DatatypeProperty ;
    rdfs:comment "Used with Work, Instance or Item" ;
    rdfs:domain bf:WorkOrInstanceOrItem ;
    rdfs:label "MARC key for X11 Names" ;
    rdfs:range rdfs:Literal ;
    skos:definition "String for name matching." .

bflc:name11MatchKey
    dcterms:modified "2017-02-02 (New)" ;
    a owl:DatatypeProperty ;
    rdfs:comment "Used with Work, Instance or Item" ;
    rdfs:domain bf:WorkOrInstanceOrItem ;
    rdfs:label "Match key for X11 Name" ;
    rdfs:range rdfs:Literal ;
    skos:definition "String for name matching." .

bflc:nonSortNum
    dcterms:modified "2022-10-04 (New [GH17])" ;
    a owl:DatatypeProperty ;
    rdfs:comment "Used with Work, Instance or Item" ;
    rdfs:domain bf:WorkOrInstanceOrItem ;
    rdfs:label "Non-sort character count" ;
    rdfs:range rdfs:Literal ;
    skos:definition "Number of characters at the start of a label that should be skipped for indexing and sorting." .

bflc:primaryContributorName00MatchKey
    dcterms:modified "2017-02-02 (New)" ;
    a owl:DatatypeProperty ;
    rdfs:comment "Used with Work, Instance or Item" ;
    rdfs:domain bf:WorkOrInstanceOrItem ;
    rdfs:label "Primary X00 Name Match key" ;
    rdfs:range rdfs:Literal ;
    skos:definition "String for entry name matching." .

bflc:primaryContributorName10MatchKey
    dcterms:modified "2017-02-02 (New)" ;
    a owl:DatatypeProperty ;
    rdfs:comment "Used with Work, Instance or Item" ;
    rdfs:domain bf:WorkOrInstanceOrItem ;
    rdfs:label "Primary X10 Name Match key" ;
    rdfs:range rdfs:Literal ;
    skos:definition "String for entry name matching." .

bflc:primaryContributorName11MatchKey
    dcterms:modified "2017-02-02 (New)" ;
    a owl:DatatypeProperty ;
    rdfs:comment "Used with Work, Instance or Item" ;
    rdfs:domain bf:WorkOrInstanceOrItem ;
    rdfs:label "Primary X11 Name Match key" ;
    rdfs:range rdfs:Literal ;
    skos:definition "String for entry name matching." .

bflc:procInfo
    dcterms:modified "2018-07-12 (New)" ;
    a owl:DatatypeProperty ;
    rdfs:domain bf:AdminMetadata ;
    rdfs:label "Processing Info" ;
    rdfs:range rdfs:Literal ;
    skos:definition "System-supplied processing information for the BIBFRAME description (e.g. \"ibc update\")." .

bflc:productionStatement
    dcterms:modified "2022-10-04 (New [GH18])" ;
    a owl:DatatypeProperty ;
    rdfs:comment "Used with Work, Instance or Item" ;
    rdfs:domain bf:WorkOrInstanceOrItem ;
    rdfs:label "Production statement" ;
    rdfs:range rdfs:Literal ;
    rdfs:subPropertyOf bflc:provisionActivityStatement ;
    skos:definition "Statement related to the production of the resource; usually transcribed." .

bflc:profile
    dcterms:modified "2018-07-12 (New)" ;
    a owl:DatatypeProperty ;
    rdfs:domain bf:AdminMetadata ;
    rdfs:label "LC Editor profile" ;
    rdfs:range rdfs:Literal ;
    skos:definition "Name of the BIBFRAME editor profile used to create or edit the description." .

bflc:projectedProvisionDate
    dcterms:modified "2017-02-02 (New)" ;
    a owl:ObjectProperty ;
    rdfs:comment "Used with Work, Instance or Item" ;
    rdfs:domain bf:WorkOrInstanceOrItem ;
    rdfs:label "Projected publication date" ;
    rdfs:range bflc:date ;
    skos:definition "Projected date of publication of the resource." .

bflc:publicationStatement
    dcterms:modified "2022-10-04 (New [GH18])" ;
    a owl:DatatypeProperty ;
    rdfs:comment "Used with Work, Instance or Item" ;
    rdfs:domain bf:WorkOrInstanceOrItem ;
    rdfs:label "Publication statement" ;
    rdfs:range rdfs:Literal ;
    rdfs:subPropertyOf bflc:provisionActivityStatement ;
    skos:definition "Statement related to the publication of the resource; ususally transcribed." .

bflc:readMarc382
    dcterms:modified "2021-11-02 (New [GH12])" ;
    a owl:ObjectProperty ;
    rdfs:comment "Used with Work, Instance or Item" ;
    rdfs:domain bf:WorkOrInstanceOrItem ;
    rdfs:label "Read-only 382 field" ;
    skos:definition "String representing the medium of performance information located in the 382 field of the original MARC record" .

bflc:relation
    dcterms:modified "2017-02-02 (New)" ;
    a owl:ObjectProperty ;
    rdfs:comment "Used with Work, Instance or Item" ;
    rdfs:domain bf:WorkOrInstanceOrItem ;
    rdfs:label "Specific relationship" ;
    rdfs:range bflc:Relation ;
    skos:definition "Connection between resources." .

bflc:relationship
    dcterms:modified "2017-02-02 (New)" ;
    a owl:ObjectProperty ;
    rdfs:comment "Used with Work, Instance or Item" ;
    rdfs:domain bf:WorkOrInstanceOrItem ;
    rdfs:label "Related resource and relationship" ;
    rdfs:range bflc:Relationship ;
    skos:definition "Resource and its connection to another resource." .

bflc:relief
    dcterms:modified "2019-05-07 (New [GH13])" ;
    a owl:ObjectProperty ;
    rdfs:comment "Used with Work, Instance or Item" ;
    rdfs:domain bf:WorkOrInstanceOrItem ;
    rdfs:label "Relief" ;
    rdfs:range bflc:Relief ;
    skos:definition "Relief term specified on a cartographic resource" .

bflc:serialPubType
    dcterms:modified "2020-03-18 (New [GH11])" ;
    a owl:ObjectProperty ;
    rdfs:comment "Used with Work, Instance or Item" ;
    rdfs:domain bf:WorkOrInstanceOrItem ;
    rdfs:label "Serial publication type" ;
    rdfs:range bflc:SerialPubType ;
    skos:definition "Information recording the type of continuing resource." .

bflc:seriesTreatment
    dcterms:modified "2018-10-12 (New)" ;
    a owl:ObjectProperty ;
    rdfs:comment "Used with Work, Instance or Item" ;
    rdfs:domain bf:WorkOrInstanceOrItem ;
    rdfs:label "Series treatment" ;
    rdfs:range bflc:SeriesTreatment ;
    skos:definition "Information concerning the treatment of a series in a resource" .

bflc:simpleAgent
    dcterms:modified "2022-10-03 (New [GH14])" ;
    a owl:DatatypeProperty ;
    rdfs:comment "Used with Work, Instance or Item" ;
    rdfs:domain bf:WorkOrInstanceOrItem ;
    rdfs:label "Agent" ;
    rdfs:range rdfs:Literal ;
    skos:definition "Name of publisher, distributor, manufacturer or producer as transcribed from the resource" .

bflc:simpleDate
    dcterms:modified "2022-10-03 (New [GH14])" ;
    a owl:DatatypeProperty ;
    rdfs:comment "Used with Work, Instance or Item" ;
    rdfs:domain bf:WorkOrInstanceOrItem ;
    rdfs:label "Date" ;
    rdfs:range rdfs:Literal ;
    skos:definition "Date of publication, distribution, manufacture or production as transcribed from the resource" .

bflc:simplePlace
    dcterms:modified "2022-10-03 (New [GH14])" ;
    a owl:DatatypeProperty ;
    rdfs:comment "Used with Work, Instance or Item" ;
    rdfs:domain bf:WorkOrInstanceOrItem ;
    rdfs:label "Place" ;
    rdfs:range rdfs:Literal ;
    skos:definition "Location of publication, distribution, manufacture or production as transcribed from the resource" .

bflc:title00MarcKey
    dcterms:modified "2017-02-02 (New)" ;
    a owl:DatatypeProperty ;
    rdfs:comment "Used with Work, Instance or Item" ;
    rdfs:domain bf:WorkOrInstanceOrItem ;
    rdfs:label "title00MarcKey" ;
    rdfs:range rdfs:Literal ;
    skos:definition "String for title matching." .

bflc:title00MatchKey
    dcterms:modified "2017-02-02 (New)" ;
    a owl:DatatypeProperty ;
    rdfs:comment "Used with Work, Instance or Item" ;
    rdfs:domain bf:WorkOrInstanceOrItem ;
    rdfs:label "Match key for Title X00" ;
    rdfs:range rdfs:Literal ;
    skos:definition "String for title matching." .

bflc:title10MarcKey
    dcterms:modified "2017-02-02 (New)" ;
    a owl:DatatypeProperty ;
    rdfs:comment "Used with Work, Instance or Item" ;
    rdfs:domain bf:WorkOrInstanceOrItem ;
    rdfs:label "title10MarcKey" ;
    rdfs:range rdfs:Literal ;
    skos:definition "String for title matching." .

bflc:title10MatchKey
    dcterms:modified "2017-02-02 (New)" ;
    a owl:DatatypeProperty ;
    rdfs:comment "Used with Work, Instance or Item" ;
    rdfs:domain bf:WorkOrInstanceOrItem ;
    rdfs:label "Match key for Title X10" ;
    rdfs:range rdfs:Literal ;
    skos:definition "String for title matching." .

bflc:title11MarcKey
    dcterms:modified "2017-02-02 (New)" ;
    a owl:DatatypeProperty ;
    rdfs:comment "Used with Work, Instance or Item" ;
    rdfs:domain bf:WorkOrInstanceOrItem ;
    rdfs:label "title11MarcKey" ;
    rdfs:range rdfs:Literal ;
    skos:definition "String for title matching." .

bflc:title11MatchKey
    dcterms:modified "2017-02-02 (New)" ;
    a owl:DatatypeProperty ;
    rdfs:comment "Used with Work, Instance or Item" ;
    rdfs:domain bf:WorkOrInstanceOrItem ;
    rdfs:label "Match key for Title X11" ;
    rdfs:range rdfs:Literal ;
    skos:definition "String for title matching." .

bflc:title30MarcKey
    dcterms:modified "2017-02-02 (New)" ;
    a owl:DatatypeProperty ;
    rdfs:comment "Used with Work, Instance or Item" ;
    rdfs:domain bf:WorkOrInstanceOrItem ;
    rdfs:label "title30MarcKey" ;
    rdfs:range rdfs:Literal ;
    skos:definition "String for title matching." .

bflc:title30MatchKey
    dcterms:modified "2017-02-02 (New)" ;
    a owl:DatatypeProperty ;
    rdfs:comment "Used with Work, Instance or Item" ;
    rdfs:domain bf:WorkOrInstanceOrItem ;
    rdfs:label "title30MatchKey" ;
    rdfs:range rdfs:Literal ;
    skos:definition "String for title matching." .

bflc:title40MatchKey
    dcterms:modified "2017-02-02 (New)" ;
    a owl:DatatypeProperty ;
    rdfs:comment "Used with Work, Instance or Item" ;
    rdfs:domain bf:WorkOrInstanceOrItem ;
    rdfs:label "title40MatchKey" ;
    rdfs:range rdfs:Literal ;
    skos:definition "String for title matching." .

