<rdf:RDF xml:base="http://id.loc.gov/ontologies/bflc/" xmlns:rdf="http://www.w3.org/1999/02/22-rdf-syntax-ns#" xmlns:rdfs="http://www.w3.org/2000/01/rdf-schema#" xmlns:bf="http://id.loc.gov/ontologies/bibframe/" xmlns:bflc="http://id.loc.gov/ontologies/bflc/" xmlns:owl="http://www.w3.org/2002/07/owl#" xmlns:skos="http://www.w3.org/2004/02/skos/core#" xmlns:dcterms="http://purl.org/dc/terms/" xmlns:foaf="http://xmlns.com/foaf/0.1/" xmlns:cc="http://creativecommons.org/ns#">
  <owl:Ontology rdf:about="">
    <owl:versionInfo rdf:datatype="http://www.w3.org/2001/XMLSchema#string">2.2.0</owl:versionInfo>
    <owl:ontologyIRI rdf:resource="http://id.loc.gov/ontologies/bflc/"/>
    <owl:versionIRI rdf:resource="http://id.loc.gov/ontologies/bflc-2-2-0/"/>
    <owl:priorVersion rdf:resource="http://id.loc.gov/ontologies/bflc-1-2-0/"/>
    <rdfs:label>BIBFRAME vocabulary with LC extensions</rdfs:label>
    <dcterms:issued rdf:datatype="http://www.w3.org/2001/XMLSchema#dateTime">2022-10-06T12:00:00.000-05:00</dcterms:issued>
    <dcterms:modified>2022-10-07T12:17:40.528-04:00</dcterms:modified>
    <dcterms:creator rdfs:resource="http://id.loc.gov/vocabulary/organizations/dlc"/>
    <dcterms:publisher rdfs:resource="http://id.loc.gov/vocabulary/organizations/dlcmrc"/>
    <dcterms:rights rdf:resource="https://creativecommons.org/publicdomain/zero/1.0/"/>
    <cc:license rdf:resource="https://creativecommons.org/publicdomain/zero/1.0/"/>
    <owl:imports rdf:resource="http://id.loc.gov/vocabulary/relators"/>
    <owl:imports rdf:resource="http://id.loc.gov/ontologies/bibframe"/>
  </owl:Ontology>
  <owl:Class rdf:about="http://id.loc.gov/ontologies/bflc/PrimaryContribution">
    <rdfs:label>Primary contribution</rdfs:label>
    <rdfs:subClassOf rdf:resource="http://id.loc.gov/ontologies/bibframe/Contribution"/>
    <skos:definition>Contribution for which the agent is the name chosen as the name part of the name and title access point.</skos:definition>
    <dcterms:modified>2017-02-02 (New)</dcterms:modified>
  </owl:Class>
  <owl:Class rdf:about="http://id.loc.gov/ontologies/bflc/Relationship">
    <rdfs:label>Relationship</rdfs:label>
    <skos:definition>Resource and its connection to another resource.</skos:definition>
    <dcterms:modified>2017-02-02 (New)</dcterms:modified>
  </owl:Class>
  <owl:Class rdf:about="http://id.loc.gov/ontologies/bflc/TransliteratedTitle">
    <rdfs:label>Transliterated title</rdfs:label>
    <rdfs:subClassOf rdf:resource="http://id.loc.gov/ontologies/bibframe/VariantTitle"/>
    <skos:definition>Title transliterated from one script to another.</skos:definition>
    <dcterms:modified>2018-07-12 (New)</dcterms:modified>
  </owl:Class>
  <owl:Class rdf:about="http://id.loc.gov/ontologies/bflc/DemographicGroup">
    <rdfs:label>Demographic group</rdfs:label>
    <skos:definition>Characteristics of a group of agents.</skos:definition>
    <dcterms:modified>2017-02-02 (New)</dcterms:modified>
  </owl:Class>
  <owl:Class rdf:about="http://id.loc.gov/ontologies/bflc/CreatorCharacteristic">
    <rdfs:label>Creator characteristic</rdfs:label>
    <skos:definition>Category to which the creators of the resource belong.</skos:definition>
    <dcterms:modified>2017-02-02 (New)</dcterms:modified>
  </owl:Class>
  <owl:Class rdf:about="http://id.loc.gov/ontologies/bflc/SeriesTreatment">
    <rdfs:label>Series treatment</rdfs:label>
    <skos:definition>Technical specification relating to the encoding of series data in a resource</skos:definition>
    <dcterms:modified>2018-10-12 (New)</dcterms:modified>
  </owl:Class>
  <owl:Class rdf:about="http://id.loc.gov/ontologies/bflc/SeriesSequentialDesignation">
    <rdfs:label>Series sequential designation</rdfs:label>
    <rdfs:subClassOf rdf:resource="http://id.loc.gov/ontologies/bflc/SeriesTreatment"/>
    <skos:definition>Beginning/ending date(s) of publication and/or sequential designations used in the bf:title field for a work. May also include a citation for the source of information.</skos:definition>
    <dcterms:modified>2018-10-12 (New)</dcterms:modified>
  </owl:Class>
  <owl:Class rdf:about="http://id.loc.gov/ontologies/bflc/SeriesNumberingPeculiarities">
    <rdfs:label>Series numbering peculiarities</rdfs:label>
    <rdfs:subClassOf rdf:resource="http://id.loc.gov/ontologies/bflc/SeriesTreatment"/>
    <skos:definition>Listing of irregularities in the report year coverage and/or numbering used in the bf:title field for a work. May also include a citation for the source of information.</skos:definition>
    <dcterms:modified>2018-10-12 (New)</dcterms:modified>
  </owl:Class>
  <owl:Class rdf:about="http://id.loc.gov/ontologies/bflc/SeriesNumbering">
    <rdfs:label>Series numbering</rdfs:label>
    <rdfs:subClassOf rdf:resource="http://id.loc.gov/ontologies/bflc/SeriesTreatment"/>
    <skos:definition>Sequential designation or numbering used in the bf:title field for a work.</skos:definition>
    <dcterms:modified>2018-10-12 (New)</dcterms:modified>
  </owl:Class>
  <owl:Class rdf:about="http://id.loc.gov/ontologies/bflc/SeriesProvider">
    <rdfs:label>Series provider</rdfs:label>
    <rdfs:subClassOf rdf:resource="http://id.loc.gov/ontologies/bflc/SeriesTreatment"/>
    <skos:definition>Place of publication and the name of the publisher/issuing body used in the bf:title field for a work.</skos:definition>
    <dcterms:modified>2018-10-12 (New)</dcterms:modified>
  </owl:Class>
  <owl:Class rdf:about="http://id.loc.gov/ontologies/bflc/SeriesAnalysis">
    <rdfs:label>Series analysis</rdfs:label>
    <rdfs:subClassOf rdf:resource="http://id.loc.gov/ontologies/bflc/SeriesTreatment"/>
    <skos:definition>A specific organization's analysis practice for a series named in the bf:title field for a work. May also contain the volumes/dates and/or the institution/copy identification to which the practice applies.</skos:definition>
    <dcterms:modified>2018-10-12 (New)</dcterms:modified>
  </owl:Class>
  <owl:Class rdf:about="http://id.loc.gov/ontologies/bflc/SeriesTracing">
    <rdfs:label>Series tracing</rdfs:label>
    <rdfs:subClassOf rdf:resource="http://id.loc.gov/ontologies/bflc/SeriesTreatment"/>
    <skos:definition>A specific organization's tracing practice for a series named in the bf:title field for a work. May also contain the volumes/dates and/or the institution/copy identification to which the practice applies.</skos:definition>
    <dcterms:modified>2018-10-12 (New)</dcterms:modified>
  </owl:Class>
  <owl:Class rdf:about="http://id.loc.gov/ontologies/bflc/SeriesClassification">
    <rdfs:label>Series classification</rdfs:label>
    <rdfs:subClassOf rdf:resource="http://id.loc.gov/ontologies/bflc/SeriesTreatment"/>
    <skos:definition>A specific organization's classification practice for a series named in the bf:title field for a work. May also contain the volumes/dates and/or the institution/copy identification to which the practice applies.</skos:definition>
    <dcterms:modified>2018-10-12 (New)</dcterms:modified>
  </owl:Class>
  <owl:Class rdf:about="http://id.loc.gov/ontologies/bflc/MovingImageTechnique">
    <rdfs:label>Moving Image Technique</rdfs:label>
    <skos:definition>Specifies the technique used in creating motion in motion pictures or videorecordings.</skos:definition>
    <dcterms:modified>2020-02-13 (New [GH9])</dcterms:modified>
  </owl:Class>
  <owl:Class rdf:about="http://id.loc.gov/ontologies/bflc/GovernmentPubType">
    <rdfs:label>Government Publication Type</rdfs:label>
    <skos:definition>Information recording that the resource is published or produced by or for an international, national, state, provincial, or local government agency, or by any subdivision of such a body.</skos:definition>
    <dcterms:modified>2020-03-09 (New [GH10])</dcterms:modified>
  </owl:Class>
  <owl:Class rdf:about="http://id.loc.gov/ontologies/bflc/SerialPubType">
    <rdfs:label>Serial Publication Type</rdfs:label>
    <skos:definition>Information recording the type of continuing resource.</skos:definition>
    <dcterms:modified>2020-03-18 (New [GH11])</dcterms:modified>
  </owl:Class>
  <owl:Class rdf:about="http://id.loc.gov/ontologies/bflc/Relief">
    <rdfs:label>Relief</rdfs:label>
    <skos:definition>Relief term specified on a cartographic resource</skos:definition>
    <dcterms:modified>2019-05-07 (New [GH13])</dcterms:modified>
  </owl:Class>
  <owl:Class rdf:about="http://id.loc.gov/ontologies/bflc/CaptureStorage">
    <rdfs:label>Capture and Storage Technique</rdfs:label>
    <rdfs:subClassOf rdf:resource="http://id.loc.gov/ontologies/bibframe/SoundCharacteristic"/>
    <skos:definition>Specifies the sound capture and storage technique used on a sound recording resource.</skos:definition>
    <dcterms:modified>2019-05-20 (New [GH16])</dcterms:modified>
  </owl:Class>
  <owl:Class rdf:about="http://id.loc.gov/ontologies/bflc/MachineModel">
    <rdfs:label>Model</rdfs:label>
    <rdfs:subClassOf rdf:resource="http://id.loc.gov/ontologies/bibframe/SystemRequirement"/>
    <skos:definition>Model of the computing device on which the resource operates.</skos:definition>
    <dcterms:modified>2017-02-02 (New)</dcterms:modified>
  </owl:Class>
  <owl:Class rdf:about="http://id.loc.gov/ontologies/bflc/ProgrammingLanguage">
    <rdfs:label>Programming language</rdfs:label>
    <rdfs:subClassOf rdf:resource="http://id.loc.gov/ontologies/bibframe/SystemRequirement"/>
    <skos:definition>Name of the programming language associated with the data comprising the resource.</skos:definition>
    <dcterms:modified>2017-02-02 (New)</dcterms:modified>
  </owl:Class>
  <owl:Class rdf:about="http://id.loc.gov/ontologies/bflc/OperatingSystem">
    <rdfs:label>Operating system</rdfs:label>
    <rdfs:subClassOf rdf:resource="http://id.loc.gov/ontologies/bibframe/SystemRequirement"/>
    <skos:definition>Software that directly operates a system's hardware and serves as a platform for applications.</skos:definition>
    <dcterms:modified>2017-02-02 (New)</dcterms:modified>
  </owl:Class>
  <owl:Class rdf:about="http://id.loc.gov/ontologies/bflc/ImageBitDepth">
    <rdfs:label>Image bit depth</rdfs:label>
    <rdfs:subClassOf rdf:resource="http://id.loc.gov/ontologies/bibframe/DigitalCharacteristic"/>
    <skos:definition>The number of bits used to represent each pixel in an image.</skos:definition>
    <dcterms:modified>2017-02-02 (New)</dcterms:modified>
  </owl:Class>
  <owl:Class rdf:about="http://id.loc.gov/ontologies/bflc/GrooveCutting">
    <rdfs:label>Groove cutting</rdfs:label>
    <rdfs:subClassOf rdf:resource="http://id.loc.gov/ontologies/bibframe/SoundCharacteristic"/>
    <skos:definition>Kind of cutting of the grooves used on a disc whose sound reproduction process involves a cutting head inscribing a modulated groove into the surface of a rotating cylinder or disc.</skos:definition>
    <dcterms:modified>2018-07-12 (New)</dcterms:modified>
  </owl:Class>
  <owl:Class rdf:about="http://id.loc.gov/ontologies/bflc/MetadataLicensor">
    <rdfs:label>Metadata licensor</rdfs:label>
    <rdfs:subClassOf rdf:resource="http://id.loc.gov/ontologies/bibframe/Agent"/>
    <skos:definition>Organization that licenses the intellectual property rights to the data contained in the description.</skos:definition>
    <dcterms:modified>2017-02-02 (New)</dcterms:modified>
  </owl:Class>
  <owl:Class rdf:about="http://id.loc.gov/ontologies/bflc/EncodingLevel">
    <rdfs:label>Encoding level</rdfs:label>
    <skos:definition>Designation of the fullness of the bibliographic description.</skos:definition>
    <dcterms:modified>2017-02-02 (New)</dcterms:modified>
  </owl:Class>
  <owl:Class rdf:about="http://id.loc.gov/ontologies/bflc/Relation">
    <rdfs:label>Relation</rdfs:label>
    <skos:definition>Connection between resources.</skos:definition>
    <dcterms:modified>2017-02-02 (New)</dcterms:modified>
  </owl:Class>
  <owl:Class rdf:about="http://id.loc.gov/ontologies/bflc/AppliesTo">
    <rdfs:label>Applies to</rdfs:label>
    <skos:definition>The component of a resource to which a characteristic applies.</skos:definition>
    <dcterms:modified>2017-02-02 (New)</dcterms:modified>
  </owl:Class>
  <owl:Class rdf:about="http://id.loc.gov/ontologies/bflc/Uncontrolled">
    <rdfs:label>Uncontrolled</rdfs:label>
    <skos:definition>Component of the resource that is not under authority control</skos:definition>
    <dcterms:modified>2021-11-02 (New [GH15])</dcterms:modified>
  </owl:Class>
  <owl:Class rdf:about="http://id.loc.gov/ontologies/bflc/Deprecated">
    <rdfs:label>Deprecated</rdfs:label>
    <skos:definition>The resource has been deprecated</skos:definition>
    <dcterms:modified>2022-10-03 (New [GH6])</dcterms:modified>
  </owl:Class>
  <owl:ObjectProperty rdf:about="http://id.loc.gov/ontologies/bflc/demographicGroup">
    <rdfs:range rdf:resource="http://id.loc.gov/ontologies/bflc/DemographicGroup"/>
    <skos:definition>Characteristics of a group of agents.</skos:definition>
    <rdfs:comment>Used with Work, Instance or Item</rdfs:comment>
    <rdfs:label>Demographic group</rdfs:label>
    <dcterms:modified>2017-02-02 (New)</dcterms:modified>
  </owl:ObjectProperty>
  <owl:ObjectProperty rdf:about="http://id.loc.gov/ontologies/bflc/creatorCharacteristic">
    <rdfs:range rdf:resource="http://id.loc.gov/ontologies/bflc/CreatorCharacteristic"/>
    <skos:definition>Category to which the creators of the resource belong.</skos:definition>
    <rdfs:comment>Used with Work, Instance or Item</rdfs:comment>
    <rdfs:label>Creator characteristic</rdfs:label>
    <dcterms:modified>2017-02-02 (New)</dcterms:modified>
  </owl:ObjectProperty>
  <owl:ObjectProperty rdf:about="http://id.loc.gov/ontologies/bflc/seriesTreatment">
    <rdfs:range rdf:resource="http://id.loc.gov/ontologies/bflc/SeriesTreatment"/>
    <skos:definition>Information concerning the treatment of a series in a resource</skos:definition>
    <rdfs:comment>Used with Work, Instance or Item</rdfs:comment>
    <rdfs:label>Series treatment</rdfs:label>
    <dcterms:modified>2018-10-12 (New)</dcterms:modified>
  </owl:ObjectProperty>
  <owl:ObjectProperty rdf:about="http://id.loc.gov/ontologies/bflc/movingImageTechnique">
    <rdfs:range rdf:resource="http://id.loc.gov/ontologies/bflc/MovingImageTechnique"/>
    <skos:definition>Information recording the technique used in creating motion in motion pictures or videorecordings.</skos:definition>
    <rdfs:comment>Used with Work, Instance or Item</rdfs:comment>
    <rdfs:label>Moving Image Technique</rdfs:label>
    <dcterms:modified>2020-02-13 (New [GH9])</dcterms:modified>
  </owl:ObjectProperty>
  <owl:ObjectProperty rdf:about="http://id.loc.gov/ontologies/bflc/governmentPubType">
    <rdfs:range rdf:resource="http://id.loc.gov/ontologies/bflc/GovernmentPubType"/>
    <skos:definition>Information recording that the resource is published or produced by or for an international, national, state, provincial, or local government agency, or by any subdivision of such a body.</skos:definition>
    <rdfs:comment>Used with Work, Instance or Item</rdfs:comment>
    <rdfs:label>Government publication type</rdfs:label>
    <dcterms:modified>2020-03-09 (New [GH10])</dcterms:modified>
  </owl:ObjectProperty>
  <owl:ObjectProperty rdf:about="http://id.loc.gov/ontologies/bflc/serialPubType">
    <rdfs:range rdf:resource="http://id.loc.gov/ontologies/bflc/SerialPubType"/>
    <skos:definition>Information recording the type of continuing resource.</skos:definition>
    <rdfs:comment>Used with Work, Instance or Item</rdfs:comment>
    <rdfs:label>Serial publication type</rdfs:label>
    <dcterms:modified>2020-03-18 (New [GH11])</dcterms:modified>
  </owl:ObjectProperty>
  <owl:ObjectProperty rdf:about="http://id.loc.gov/ontologies/bflc/readMarc382">
    <skos:definition>String representing the medium of performance information located in the 382 field of the original MARC record</skos:definition>
    <rdfs:comment>Used with Work, Instance or Item</rdfs:comment>
    <rdfs:label>Read-only 382 field</rdfs:label>
    <dcterms:modified>2021-11-02 (New [GH12])</dcterms:modified>
  </owl:ObjectProperty>
  <owl:ObjectProperty rdf:about="http://id.loc.gov/ontologies/bflc/projectedProvisionDate">
    <rdfs:range rdf:resource="http://id.loc.gov/ontologies/bflc/date"/>
    <skos:definition>Projected date of publication of the resource.</skos:definition>
    <rdfs:comment>Used with Work, Instance or Item</rdfs:comment>
    <rdfs:label>Projected publication date</rdfs:label>
    <dcterms:modified>2017-02-02 (New)</dcterms:modified>
  </owl:ObjectProperty>
  <owl:ObjectProperty rdf:about="http://id.loc.gov/ontologies/bflc/relief">
    <rdfs:range rdf:resource="http://id.loc.gov/ontologies/bflc/Relief"/>
    <skos:definition>Relief term specified on a cartographic resource</skos:definition>
    <rdfs:comment>Used with Work, Instance or Item</rdfs:comment>
    <rdfs:label>Relief</rdfs:label>
    <dcterms:modified>2019-05-07 (New [GH13])</dcterms:modified>
  </owl:ObjectProperty>
  <owl:DatatypeProperty rdf:about="http://id.loc.gov/ontologies/bflc/simpleAgent">
    <rdfs:range rdf:resource="http://www.w3.org/2000/01/rdf-schema#Literal"/>
    <skos:definition>Name of publisher, distributor, manufacturer or producer as transcribed from the resource</skos:definition>
    <rdfs:comment>Used with Work, Instance or Item</rdfs:comment>
    <rdfs:label>Agent</rdfs:label>
    <dcterms:modified>2022-10-03 (New [GH14])</dcterms:modified>
  </owl:DatatypeProperty>
  <owl:DatatypeProperty rdf:about="http://id.loc.gov/ontologies/bflc/simpleDate">
    <rdfs:range rdf:resource="http://www.w3.org/2000/01/rdf-schema#Literal"/>
    <skos:definition>Date of publication, distribution, manufacture or production as transcribed from the resource</skos:definition>
    <rdfs:comment>Used with Work, Instance or Item</rdfs:comment>
    <rdfs:label>Date</rdfs:label>
    <dcterms:modified>2022-10-03 (New [GH14])</dcterms:modified>
  </owl:DatatypeProperty>
  <owl:DatatypeProperty rdf:about="http://id.loc.gov/ontologies/bflc/simplePlace">
    <rdfs:range rdf:resource="http://www.w3.org/2000/01/rdf-schema#Literal"/>
    <skos:definition>Location of publication, distribution, manufacture or production as transcribed from the resource</skos:definition>
    <rdfs:comment>Used with Work, Instance or Item</rdfs:comment>
    <rdfs:label>Place</rdfs:label>
    <dcterms:modified>2022-10-03 (New [GH14])</dcterms:modified>
  </owl:DatatypeProperty>
  <owl:DatatypeProperty rdf:about="http://id.loc.gov/ontologies/bflc/distributionStatement">
    <rdfs:range rdf:resource="http://www.w3.org/2000/01/rdf-schema#Literal"/>
    <skos:definition>Statement related to the distribution of the resource; usually transcribed.</skos:definition>
    <rdfs:subPropertyOf rdf:resource="http://id.loc.gov/ontologies/bflc/provisionActivityStatement"/>
    <rdfs:comment>Used with Work, Instance or Item</rdfs:comment>
    <rdfs:label>Distribution statement</rdfs:label>
    <dcterms:modified>2022-10-04 (New [GH18])</dcterms:modified>
  </owl:DatatypeProperty>
  <owl:DatatypeProperty rdf:about="http://id.loc.gov/ontologies/bflc/manufactureStatement">
    <rdfs:range rdf:resource="http://www.w3.org/2000/01/rdf-schema#Literal"/>
    <skos:definition>Statement related to the manufacture of the resource; usually transcribed.</skos:definition>
    <rdfs:subPropertyOf rdf:resource="http://id.loc.gov/ontologies/bflc/provisionActivityStatement"/>
    <rdfs:comment>Used with Work, Instance or Item</rdfs:comment>
    <rdfs:label>Manufacture statement</rdfs:label>
    <dcterms:modified>2022-10-04 (New [GH18])</dcterms:modified>
  </owl:DatatypeProperty>
  <owl:DatatypeProperty rdf:about="http://id.loc.gov/ontologies/bflc/productionStatement">
    <rdfs:range rdf:resource="http://www.w3.org/2000/01/rdf-schema#Literal"/>
    <skos:definition>Statement related to the production of the resource; usually transcribed.</skos:definition>
    <rdfs:subPropertyOf rdf:resource="http://id.loc.gov/ontologies/bflc/provisionActivityStatement"/>
    <rdfs:comment>Used with Work, Instance or Item</rdfs:comment>
    <rdfs:label>Production statement</rdfs:label>
    <dcterms:modified>2022-10-04 (New [GH18])</dcterms:modified>
  </owl:DatatypeProperty>
  <owl:DatatypeProperty rdf:about="http://id.loc.gov/ontologies/bflc/publicationStatement">
    <rdfs:range rdf:resource="http://www.w3.org/2000/01/rdf-schema#Literal"/>
    <skos:definition>Statement related to the publication of the resource; ususally transcribed.</skos:definition>
    <rdfs:subPropertyOf rdf:resource="http://id.loc.gov/ontologies/bflc/provisionActivityStatement"/>
    <rdfs:comment>Used with Work, Instance or Item</rdfs:comment>
    <rdfs:label>Publication statement</rdfs:label>
    <dcterms:modified>2022-10-04 (New [GH18])</dcterms:modified>
  </owl:DatatypeProperty>
  <owl:ObjectProperty rdf:about="http://id.loc.gov/ontologies/bflc/indexedIn">
    <skos:definition>Citation to the resource where the material being described is indexed.</skos:definition>
    <rdfs:comment>Used with Work, Instance or Item</rdfs:comment>
    <rdfs:label>Indexed in</rdfs:label>
    <dcterms:modified>2018-07-12 (New)</dcterms:modified>
  </owl:ObjectProperty>
  <owl:ObjectProperty rdf:about="http://id.loc.gov/ontologies/bflc/metadataLicensor">
    <rdfs:domain rdf:resource="http://id.loc.gov/ontologies/bflc/bf:AdminMetadata"/>
    <rdfs:range rdf:resource="http://id.loc.gov/ontologies/bflc/MetadataLicensor"/>
    <skos:definition>Organization that licenses the intellectual property rights to the data contained in the description.</skos:definition>
    <rdfs:label>Metadata licensor</rdfs:label>
    <dcterms:modified>2017-02-02 (New)</dcterms:modified>
  </owl:ObjectProperty>
  <owl:ObjectProperty rdf:about="http://id.loc.gov/ontologies/bflc/encodingLevel">
    <rdfs:domain rdf:resource="http://id.loc.gov/ontologies/bflc/bf:AdminMetadata"/>
    <rdfs:range rdf:resource="http://id.loc.gov/ontologies/bflc/EncodingLevel"/>
    <skos:definition>Designation of the fullness of the bibliographic description.</skos:definition>
    <rdfs:label>Encoding level</rdfs:label>
    <dcterms:modified>2017-02-02 (New)</dcterms:modified>
  </owl:ObjectProperty>
  <owl:DatatypeProperty rdf:about="http://id.loc.gov/ontologies/bflc/catalogerId">
    <rdfs:domain rdf:resource="http://id.loc.gov/ontologies/bflc/bf:AdminMetadata"/>
    <rdfs:range rdf:resource="http://www.w3.org/2000/01/rdf-schema#Literal"/>
    <skos:definition>ID of the cataloger who created or edited the description.</skos:definition>
    <rdfs:label>Cataloger ID</rdfs:label>
    <dcterms:modified>2018-07-12 (New)</dcterms:modified>
  </owl:DatatypeProperty>
  <owl:DatatypeProperty rdf:about="http://id.loc.gov/ontologies/bflc/profile">
    <rdfs:domain rdf:resource="http://id.loc.gov/ontologies/bflc/bf:AdminMetadata"/>
    <rdfs:range rdf:resource="http://www.w3.org/2000/01/rdf-schema#Literal"/>
    <skos:definition>Name of the BIBFRAME editor profile used to create or edit the description.</skos:definition>
    <rdfs:label>LC Editor profile</rdfs:label>
    <dcterms:modified>2018-07-12 (New)</dcterms:modified>
  </owl:DatatypeProperty>
  <owl:DatatypeProperty rdf:about="http://id.loc.gov/ontologies/bflc/procInfo">
    <rdfs:domain rdf:resource="http://id.loc.gov/ontologies/bflc/bf:AdminMetadata"/>
    <rdfs:range rdf:resource="http://www.w3.org/2000/01/rdf-schema#Literal"/>
    <skos:definition>System-supplied processing information for the BIBFRAME description (e.g. "ibc update").</skos:definition>
    <rdfs:label>Processing Info</rdfs:label>
    <dcterms:modified>2018-07-12 (New)</dcterms:modified>
  </owl:DatatypeProperty>
  <owl:ObjectProperty rdf:about="http://id.loc.gov/ontologies/bflc/appliesTo">
    <rdfs:range rdf:resource="http://id.loc.gov/ontologies/bflc/AppliesTo"/>
    <skos:definition>The component of a resource to which a characteristic applies.</skos:definition>
    <rdfs:comment>Used with Work, Instance or Item</rdfs:comment>
    <rdfs:label>Applies to</rdfs:label>
    <dcterms:modified>2017-02-02 (New)</dcterms:modified>
  </owl:ObjectProperty>
  <owl:ObjectProperty rdf:about="http://id.loc.gov/ontologies/bflc/applicableInstitution">
    <rdfs:range rdf:resource="http://id.loc.gov/ontologies/bibframe/Agent"/>
    <skos:definition>Institutional location of a resource to which a particular piece of description applies.</skos:definition>
    <rdfs:comment>Used with Work, Instance or Item</rdfs:comment>
    <rdfs:label>Applicable institution</rdfs:label>
    <dcterms:modified>2017-02-02 (New)</dcterms:modified>
  </owl:ObjectProperty>
  <owl:ObjectProperty rdf:about="http://id.loc.gov/ontologies/bflc/relationship">
    <rdfs:range rdf:resource="http://id.loc.gov/ontologies/bflc/Relationship"/>
    <skos:definition>Resource and its connection to another resource.</skos:definition>
    <rdfs:comment>Used with Work, Instance or Item</rdfs:comment>
    <rdfs:label>Related resource and relationship</rdfs:label>
    <dcterms:modified>2017-02-02 (New)</dcterms:modified>
  </owl:ObjectProperty>
  <owl:ObjectProperty rdf:about="http://id.loc.gov/ontologies/bflc/relation">
    <rdfs:range rdf:resource="http://id.loc.gov/ontologies/bflc/Relation"/>
    <skos:definition>Connection between resources.</skos:definition>
    <rdfs:comment>Used with Work, Instance or Item</rdfs:comment>
    <rdfs:label>Specific relationship</rdfs:label>
    <dcterms:modified>2017-02-02 (New)</dcterms:modified>
  </owl:ObjectProperty>
  <owl:DatatypeProperty rdf:about="http://id.loc.gov/ontologies/bflc/aap">
    <rdfs:range rdf:resource="http://www.w3.org/2000/01/rdf-schema#Literal"/>
    <skos:definition>A text string that represents the label of the resource. It could be a name/title combination, but could also include additional fields to make it unique within the catalog.</skos:definition>
    <rdfs:comment>Used with Work, Instance or Item</rdfs:comment>
    <rdfs:label>Authorized access point</rdfs:label>
    <dcterms:modified>2021-11-02 (New [GH2])</dcterms:modified>
  </owl:DatatypeProperty>
  <owl:DatatypeProperty rdf:about="http://id.loc.gov/ontologies/bflc/aap-normalized">
    <rdfs:range rdf:resource="http://www.w3.org/2000/01/rdf-schema#Literal"/>
    <skos:definition>Normalized version of the authorized access point with spaces, capitalization, and punctuation removed.</skos:definition>
    <rdfs:comment>Used with Work, Instance or Item</rdfs:comment>
    <rdfs:label>Normalized authorized access point</rdfs:label>
    <dcterms:modified>2021-11-02 (New [GH2])</dcterms:modified>
  </owl:DatatypeProperty>
  <owl:DatatypeProperty rdf:about="http://id.loc.gov/ontologies/bflc/nonSortNum">
    <rdfs:range rdf:resource="http://www.w3.org/2000/01/rdf-schema#Literal"/>
    <skos:definition>Number of characters at the start of a label that should be skipped for indexing and sorting.</skos:definition>
    <rdfs:comment>Used with Work, Instance or Item</rdfs:comment>
    <rdfs:label>Non-sort character count</rdfs:label>
    <dcterms:modified>2022-10-04 (New [GH17])</dcterms:modified>
  </owl:DatatypeProperty>
  <owl:DatatypeProperty rdf:about="http://id.loc.gov/ontologies/bflc/marcKey">
    <rdfs:range rdf:resource="http://www.w3.org/2000/01/rdf-schema#Literal"/>
    <skos:definition>String to store MARC data</skos:definition>
    <rdfs:comment>Used with Work, Instance or Item</rdfs:comment>
    <rdfs:label>MARC key for headings</rdfs:label>
    <dcterms:modified>2022-10-03 (New [GH7])</dcterms:modified>
  </owl:DatatypeProperty>
  <owl:DatatypeProperty rdf:about="http://id.loc.gov/ontologies/bflc/name00MatchKey">
    <rdfs:range rdf:resource="http://www.w3.org/2000/01/rdf-schema#Literal"/>
    <skos:definition>String for name matching.</skos:definition>
    <rdfs:comment>Used with Work, Instance or Item</rdfs:comment>
    <rdfs:label>Match key for X00 Name</rdfs:label>
    <dcterms:modified>2017-02-02 (New)</dcterms:modified>
  </owl:DatatypeProperty>
  <owl:DatatypeProperty rdf:about="http://id.loc.gov/ontologies/bflc/name10MatchKey">
    <rdfs:range rdf:resource="http://www.w3.org/2000/01/rdf-schema#Literal"/>
    <skos:definition>String for name matching.</skos:definition>
    <rdfs:comment>Used with Work, Instance or Item</rdfs:comment>
    <rdfs:label>Match key for X10 Name</rdfs:label>
    <dcterms:modified>2017-02-02 (New)</dcterms:modified>
  </owl:DatatypeProperty>
  <owl:DatatypeProperty rdf:about="http://id.loc.gov/ontologies/bflc/name11MatchKey">
    <rdfs:range rdf:resource="http://www.w3.org/2000/01/rdf-schema#Literal"/>
    <skos:definition>String for name matching.</skos:definition>
    <rdfs:comment>Used with Work, Instance or Item</rdfs:comment>
    <rdfs:label>Match key for X11 Name</rdfs:label>
    <dcterms:modified>2017-02-02 (New)</dcterms:modified>
  </owl:DatatypeProperty>
  <owl:DatatypeProperty rdf:about="http://id.loc.gov/ontologies/bflc/name00MarcKey">
    <rdfs:range rdf:resource="http://www.w3.org/2000/01/rdf-schema#Literal"/>
    <skos:definition>String for personal name matching.</skos:definition>
    <rdfs:comment>Used with Work, Instance or Item</rdfs:comment>
    <rdfs:label>MARC key for X00 Names</rdfs:label>
    <dcterms:modified>2017-02-02 (New)</dcterms:modified>
  </owl:DatatypeProperty>
  <owl:DatatypeProperty rdf:about="http://id.loc.gov/ontologies/bflc/name10MarcKey">
    <rdfs:range rdf:resource="http://www.w3.org/2000/01/rdf-schema#Literal"/>
    <skos:definition>String for name matching.</skos:definition>
    <rdfs:comment>Used with Work, Instance or Item</rdfs:comment>
    <rdfs:label>MARC key for X10 Names</rdfs:label>
    <dcterms:modified>2017-02-02 (New)</dcterms:modified>
  </owl:DatatypeProperty>
  <owl:DatatypeProperty rdf:about="http://id.loc.gov/ontologies/bflc/name11MarcKey">
    <rdfs:range rdf:resource="http://www.w3.org/2000/01/rdf-schema#Literal"/>
    <skos:definition>String for name matching.</skos:definition>
    <rdfs:comment>Used with Work, Instance or Item</rdfs:comment>
    <rdfs:label>MARC key for X11 Names</rdfs:label>
    <dcterms:modified>2017-02-02 (New)</dcterms:modified>
  </owl:DatatypeProperty>
  <owl:DatatypeProperty rdf:about="http://id.loc.gov/ontologies/bflc/primaryContributorName00MatchKey">
    <rdfs:range rdf:resource="http://www.w3.org/2000/01/rdf-schema#Literal"/>
    <skos:definition>String for entry name matching.</skos:definition>
    <rdfs:comment>Used with Work, Instance or Item</rdfs:comment>
    <rdfs:label>Primary X00 Name Match key</rdfs:label>
    <dcterms:modified>2017-02-02 (New)</dcterms:modified>
  </owl:DatatypeProperty>
  <owl:DatatypeProperty rdf:about="http://id.loc.gov/ontologies/bflc/primaryContributorName10MatchKey">
    <rdfs:range rdf:resource="http://www.w3.org/2000/01/rdf-schema#Literal"/>
    <skos:definition>String for entry name matching.</skos:definition>
    <rdfs:comment>Used with Work, Instance or Item</rdfs:comment>
    <rdfs:label>Primary X10 Name Match key</rdfs:label>
    <dcterms:modified>2017-02-02 (New)</dcterms:modified>
  </owl:DatatypeProperty>
  <owl:DatatypeProperty rdf:about="http://id.loc.gov/ontologies/bflc/primaryContributorName11MatchKey">
    <rdfs:range rdf:resource="http://www.w3.org/2000/01/rdf-schema#Literal"/>
    <skos:definition>String for entry name matching.</skos:definition>
    <rdfs:comment>Used with Work, Instance or Item</rdfs:comment>
    <rdfs:label>Primary X11 Name Match key</rdfs:label>
    <dcterms:modified>2017-02-02 (New)</dcterms:modified>
  </owl:DatatypeProperty>
  <owl:DatatypeProperty rdf:about="http://id.loc.gov/ontologies/bflc/title00MatchKey">
    <rdfs:range rdf:resource="http://www.w3.org/2000/01/rdf-schema#Literal"/>
    <skos:definition>String for title matching.</skos:definition>
    <rdfs:comment>Used with Work, Instance or Item</rdfs:comment>
    <rdfs:label>Match key for Title X00</rdfs:label>
    <dcterms:modified>2017-02-02 (New)</dcterms:modified>
  </owl:DatatypeProperty>
  <owl:DatatypeProperty rdf:about="http://id.loc.gov/ontologies/bflc/title10MatchKey">
    <rdfs:range rdf:resource="http://www.w3.org/2000/01/rdf-schema#Literal"/>
    <skos:definition>String for title matching.</skos:definition>
    <rdfs:comment>Used with Work, Instance or Item</rdfs:comment>
    <rdfs:label>Match key for Title X10</rdfs:label>
    <dcterms:modified>2017-02-02 (New)</dcterms:modified>
  </owl:DatatypeProperty>
  <owl:DatatypeProperty rdf:about="http://id.loc.gov/ontologies/bflc/title11MatchKey">
    <rdfs:range rdf:resource="http://www.w3.org/2000/01/rdf-schema#Literal"/>
    <skos:definition>String for title matching.</skos:definition>
    <rdfs:comment>Used with Work, Instance or Item</rdfs:comment>
    <rdfs:label>Match key for Title X11</rdfs:label>
    <dcterms:modified>2017-02-02 (New)</dcterms:modified>
  </owl:DatatypeProperty>
  <owl:DatatypeProperty rdf:about="http://id.loc.gov/ontologies/bflc/title30MatchKey">
    <rdfs:range rdf:resource="http://www.w3.org/2000/01/rdf-schema#Literal"/>
    <skos:definition>String for title matching.</skos:definition>
    <rdfs:comment>Used with Work, Instance or Item</rdfs:comment>
    <rdfs:label>title30MatchKey</rdfs:label>
    <dcterms:modified>2017-02-02 (New)</dcterms:modified>
  </owl:DatatypeProperty>
  <owl:DatatypeProperty rdf:about="http://id.loc.gov/ontologies/bflc/title40MatchKey">
    <rdfs:range rdf:resource="http://www.w3.org/2000/01/rdf-schema#Literal"/>
    <skos:definition>String for title matching.</skos:definition>
    <rdfs:comment>Used with Work, Instance or Item</rdfs:comment>
    <rdfs:label>title40MatchKey</rdfs:label>
    <dcterms:modified>2017-02-02 (New)</dcterms:modified>
  </owl:DatatypeProperty>
  <owl:DatatypeProperty rdf:about="http://id.loc.gov/ontologies/bflc/title00MarcKey">
    <rdfs:range rdf:resource="http://www.w3.org/2000/01/rdf-schema#Literal"/>
    <skos:definition>String for title matching.</skos:definition>
    <rdfs:comment>Used with Work, Instance or Item</rdfs:comment>
    <rdfs:label>title00MarcKey</rdfs:label>
    <dcterms:modified>2017-02-02 (New)</dcterms:modified>
  </owl:DatatypeProperty>
  <owl:DatatypeProperty rdf:about="http://id.loc.gov/ontologies/bflc/title10MarcKey">
    <rdfs:range rdf:resource="http://www.w3.org/2000/01/rdf-schema#Literal"/>
    <skos:definition>String for title matching.</skos:definition>
    <rdfs:comment>Used with Work, Instance or Item</rdfs:comment>
    <rdfs:label>title10MarcKey</rdfs:label>
    <dcterms:modified>2017-02-02 (New)</dcterms:modified>
  </owl:DatatypeProperty>
  <owl:DatatypeProperty rdf:about="http://id.loc.gov/ontologies/bflc/title11MarcKey">
    <rdfs:range rdf:resource="http://www.w3.org/2000/01/rdf-schema#Literal"/>
    <skos:definition>String for title matching.</skos:definition>
    <rdfs:comment>Used with Work, Instance or Item</rdfs:comment>
    <rdfs:label>title11MarcKey</rdfs:label>
    <dcterms:modified>2017-02-02 (New)</dcterms:modified>
  </owl:DatatypeProperty>
  <owl:DatatypeProperty rdf:about="http://id.loc.gov/ontologies/bflc/title30MarcKey">
    <rdfs:range rdf:resource="http://www.w3.org/2000/01/rdf-schema#Literal"/>
    <skos:definition>String for title matching.</skos:definition>
    <rdfs:comment>Used with Work, Instance or Item</rdfs:comment>
    <rdfs:label>title30MarcKey</rdfs:label>
    <dcterms:modified>2017-02-02 (New)</dcterms:modified>
  </owl:DatatypeProperty>
</rdf:RDF>
